In progress epoch correctness

intermediate/Veritas.Intermediate.Global.fst
@@ -13,141 +13,133 @@ let verifiable_implies_prefix_verifiable
   in
   ()
 
-let rec add_seq_aux (#vcfg:_) (gl: verifiable_log vcfg): 
+let rec add_seq (#vcfg:_) (ep: epoch) (gl: verifiable_log vcfg):
   Tot (seq (ms_hashfn_dom))
   (decreases (S.length gl)) = 
   let p = S.length gl in
   if p = 0 then S.empty #(ms_hashfn_dom)
   else
     let gl' = SA.prefix gl (p - 1) in
-    // verifiable_implies_prefix_verifiable gl (p - 1);
-    append (add_seq_aux gl') (IntT.blum_add_seq (thread_log gl (p - 1)))
+    append (add_seq ep gl') (IntT.blum_add_seq ep (thread_log gl (p - 1)))
 
-let add_seq (#vcfg:_) (gl: verifiable_log vcfg): seq (ms_hashfn_dom) = 
-  add_seq_aux gl
-
-let rec lemma_g_hadd_correct_aux #vcfg (gl: verifiable_log vcfg):
-  Lemma (ensures (hadd gl = ms_hashfn (add_seq gl)))
+let rec lemma_g_hadd_correct #vcfg (ep: epoch) (gl: verifiable_log vcfg):
+  Lemma (ensures (hadd gl ep = ms_hashfn (add_seq ep gl)))
         (decreases (S.length gl)) = 
   let p = S.length gl in
-  let s = add_seq gl in
-  let h = hadd gl in
+  let s = add_seq ep gl in
+  let h = hadd gl ep in
   if p = 0 then
     lemma_hashfn_empty()
   else (
     let gl' = SA.prefix gl (p - 1) in
-    let s' = add_seq gl' in
-    let h' = hadd gl' in
-    lemma_g_hadd_correct_aux gl';
+    let s' = add_seq ep gl' in
+    let h' = hadd gl' ep in
+    lemma_g_hadd_correct ep gl';
     assert(h' = ms_hashfn s');
 
     let tl = thread_log gl (p - 1) in
-    let st = blum_add_seq tl in
-    let ht = IntT.hadd tl in
-    IntT.lemma_hadd_correct tl;
+    let st = blum_add_seq ep tl in
+    let ht = IntT.hadd tl ep in
+    IntT.lemma_hadd_correct ep tl;
     lemma_hashfn_agg s' st
   )
 
-let lemma_g_hadd_correct (#vcfg:_) (gl: verifiable_log vcfg):
-  Lemma (ensures (hadd gl = ms_hashfn (add_seq gl))) = 
-  lemma_g_hadd_correct_aux gl
-
-let rec add_set_map_aux #vcfg (gl: verifiable_log vcfg) (ii: sseq_index gl {is_blum_add (indexss gl ii)}):
-  Tot (j: SA.seq_index (add_seq gl){S.index (add_seq gl) j = blum_add_elem (indexss gl ii)})
-  (decreases (S.length gl))  
+(* mapping from blum_add entries in verifier log to the index in add seq *)
+let rec add_set_map (#vcfg:_) (gl: verifiable_log vcfg) (ii: sseq_index gl {is_blum_add (indexss gl ii)}):
+  Tot (let e = indexss gl ii in
+   let be = blum_add_elem e in
+   let ep = epoch_of be in
+   let as = add_seq ep gl in
+   j: SA.seq_index as {S.index as j = be})
+  (decreases (S.length gl))
   = 
   let (tid, i) = ii in
+  let e = indexss gl ii in
+  let be = blum_add_elem e in
+  let ep = epoch_of be in
   let p = S.length gl in
   let gl' = SA.prefix gl (p - 1) in
-  let s' = add_seq gl' in
+  let s' = add_seq ep gl' in
   let tl = thread_log gl (p - 1) in
 
   if tid = p - 1 then
     S.length s' + (IntT.add_seq_map tl i)
   else
-    add_set_map_aux gl' ii  
+    add_set_map gl' ii
 
-(* mapping from blum_add entries in verifier log to the index in add seq *)
-let add_set_map (#vcfg:_) (gl: verifiable_log vcfg) (ii: sseq_index gl {is_blum_add (indexss gl ii)}):
-  (j: SA.seq_index (add_seq gl){S.index (add_seq gl) j = blum_add_elem (indexss gl ii)}) = 
-  add_set_map_aux gl ii
-
-let rec add_set_map_inv_aux (#vcfg:_) (gl: verifiable_log vcfg) (j: SA.seq_index (add_seq gl)):
-  Tot (ii: sseq_index gl {is_blum_add (indexss gl ii) /\ 
-                      add_set_map gl ii = j})
-  (decreases (S.length gl)) = 
+(* inverse mapping from add_seq to the blum add entries in the verifier logs *)
+let rec add_set_map_inv (#vcfg:_) (ep: epoch) (gl: verifiable_log vcfg) (j: SA.seq_index (add_seq ep gl)):
+  Tot (ii: sseq_index gl {let e = indexss gl ii in
+                      is_blum_add e /\
+                      (let be = blum_add_elem e in
+                       let as = add_seq ep gl in
+                       be = S.index as j /\
+                       add_set_map gl ii = j /\
+                       ep = epoch_of be)})
+  (decreases (S.length gl)) =
   let p = S.length gl in
   let gl' = SA.prefix gl (p - 1) in
-  let s' = add_seq gl' in
+  let s' = add_seq ep gl' in
   let tl = thread_log gl (p - 1) in
 
   if j < S.length s' then
-    add_set_map_inv_aux gl' j
+    add_set_map_inv ep gl' j
   else
     let j' = j - S.length s' in
-    let i = IntT.add_seq_inv_map tl j' in
+    let i = IntT.add_seq_inv_map ep tl j' in
     (p - 1, i)
 
-(* inverse mapping from add_seq to the blum add entries in the verifier logs *)
-let add_set_map_inv (#vcfg:_) (gl: verifiable_log vcfg) (j: SA.seq_index (add_seq gl)):
-  (ii: sseq_index gl {is_blum_add (indexss gl ii) /\ 
-                      add_set_map gl ii = j}) = add_set_map_inv_aux gl j
-
-let rec lemma_add_set_map_inv_aux (#vcfg:_) (gl: verifiable_log vcfg) (ii: sseq_index gl {is_blum_add (indexss gl ii)}):
-  Lemma (ensures (add_set_map_inv gl (add_set_map gl ii) = ii))
-        (decreases (S.length gl)) = 
+let rec lemma_add_set_map_inv (#vcfg:_) (gl: verifiable_log vcfg) (ii: sseq_index gl {is_blum_add (indexss gl ii)}):
+  Lemma (ensures (let e = indexss gl ii in
+                  let be = blum_add_elem e in
+                  let ep = epoch_of be in
+                  let j = add_set_map gl ii in
+                  add_set_map_inv ep gl j = ii))
+        (decreases (S.length gl)) =
+  let e = indexss gl ii in
+  let be = blum_add_elem e in
+  let ep = epoch_of be in
   let (tid, i) = ii in
   let p = S.length gl in
   let gl' = SA.prefix gl (p - 1) in
-  let s' = add_seq gl' in
+  let s' = add_seq ep gl' in
   let tl = thread_log gl (p - 1) in
 
   if tid = p - 1 then ()
   else
-    lemma_add_set_map_inv_aux gl' ii
-
-let lemma_add_set_map_inv (#vcfg:_) (gl: verifiable_log vcfg) (ii: sseq_index gl {is_blum_add (indexss gl ii)}):
-  Lemma (ensures (add_set_map_inv gl (add_set_map gl ii) = ii)) = lemma_add_set_map_inv_aux gl ii
+    lemma_add_set_map_inv gl' ii
 
 (* a single sequence containing all the blum evicts *)
-let rec evict_seq_aux (#vcfg:_) (gl: verifiable_log vcfg): 
+let rec evict_seq (#vcfg:_) (ep: epoch) (gl: verifiable_log vcfg):
   Tot (seq ms_hashfn_dom)
   (decreases (S.length gl)) =
   let p = S.length gl in
   if p = 0 then S.empty #(ms_hashfn_dom)
   else
     let gl' = SA.prefix gl (p - 1) in
-    append (evict_seq_aux gl') (IntT.blum_evict_seq (thread_log gl (p - 1)))
+    append (evict_seq ep gl') (IntT.blum_evict_seq ep (thread_log gl (p - 1)))
 
-(* a single sequence containing all the blum evicts *)
-let evict_seq (#vcfg:_) (gl: verifiable_log vcfg): seq ms_hashfn_dom = 
-  evict_seq_aux gl
-
-let rec lemma_ghevict_correct_aux (#vcfg:_) (gl: verifiable_log vcfg):
-  Lemma (ensures (hevict gl = ms_hashfn (evict_seq gl)))
+let rec lemma_ghevict_correct (#vcfg:_) (ep: epoch) (gl: verifiable_log vcfg):
+  Lemma (ensures (hevict gl ep = ms_hashfn (evict_seq ep gl)))
         (decreases (S.length gl)) = 
   let p = S.length gl in
-  let s = evict_seq gl in
-  let h = hevict gl in
+  let s = evict_seq ep gl in
+  let h = hevict gl ep in
   if p = 0 then
     lemma_hashfn_empty()
   else (
     let gl' = SA.prefix gl (p - 1) in
-    let s' = evict_seq gl' in
-    let h' = hevict gl' in
-    lemma_ghevict_correct_aux gl';
+    let s' = evict_seq ep gl' in
+    let h' = hevict gl' ep in
+    lemma_ghevict_correct ep gl';
     let tl = thread_log gl (p - 1) in
-    let st = IntT.blum_evict_seq tl in
-    let ht = IntT.hevict tl in
-    IntT.lemma_hevict_correct tl;
+    let st = IntT.blum_evict_seq ep tl in
+    let ht = IntT.hevict tl ep in
+    IntT.lemma_hevict_correct ep tl;
     
     lemma_hashfn_agg s' st
   )
         
-let lemma_ghevict_correct (#vcfg:_) (gl: verifiable_log vcfg):
-  Lemma (ensures (hevict gl = ms_hashfn (evict_seq gl))) =
-  lemma_ghevict_correct_aux gl
-
 (* two indexes of a sequence s are different *)
 let diff_elem (#a:eqtype) (s:seq a) (i1: SA.seq_index s) (i2: SA.seq_index s) = 
   S.index s i1 <> S.index s i2
@@ -223,149 +215,180 @@ let rec lemma_uniq_prop_counts (#a:eqtype) (s: seq a) (x: a):
 
 module MH = Veritas.MultiSetHash
 
-let rec lemma_evict_elem_tids #vcfg (gl: verifiable_log vcfg) (i: SA.seq_index (evict_seq gl))
-  : Lemma (ensures (let es = evict_seq gl in
+let rec lemma_evict_elem_tids #vcfg (ep: epoch) (gl: verifiable_log vcfg) (i: SA.seq_index (evict_seq ep gl))
+  : Lemma (ensures (let es = evict_seq ep gl in
                     MH.thread_id_of (S.index es i) < S.length gl))
           (decreases (S.length gl)) = 
   let p = S.length gl in
-  let es = evict_seq gl in
+  let es = evict_seq ep gl in
   if p = 0 then ()
   else
     let gl' = SA.prefix gl (p - 1) in
-    let es' = evict_seq gl' in
+    let es' = evict_seq ep gl' in
     if i < S.length es' then
-      lemma_evict_elem_tids gl' i
+      lemma_evict_elem_tids ep gl' i
     else      
-      IntT.lemma_evict_elem_tid (thread_log gl (p - 1))
+      IntT.lemma_evict_elem_tid ep (thread_log gl (p - 1))
 
-let rec lemma_evict_elem_unique_aux #vcfg (gl: verifiable_log vcfg) (i1 i2: SA.seq_index (evict_seq gl))
+let rec lemma_evict_elem_unique_aux #vcfg (ep: epoch) (gl: verifiable_log vcfg)
+  (i1 i2: SA.seq_index (evict_seq ep gl))
   : Lemma (requires (i1 < i2))
-          (ensures (diff_elem (evict_seq gl) i1 i2))
+          (ensures (diff_elem (evict_seq ep gl) i1 i2))
           (decreases (S.length gl)) = 
   let p = S.length gl in
-  let es = evict_seq gl in
+  let es = evict_seq ep gl in
   if p = 0 then ()
   else
     let gl' = SA.prefix gl (p - 1) in
-    let es' = evict_seq gl' in
+    let es' = evict_seq ep gl' in
     let tl = thread_log gl (p - 1) in
-    let et = IntT.blum_evict_seq tl in
+    let et = IntT.blum_evict_seq ep tl in
     if i1 < S.length es' then
       if i2 < S.length es' then
-        lemma_evict_elem_unique_aux gl' i1 i2
+        lemma_evict_elem_unique_aux ep gl' i1 i2
       else (
-        lemma_evict_elem_tids gl' i1; 
-        IntT.lemma_evict_elem_tid tl
+        lemma_evict_elem_tids ep gl' i1;
+        IntT.lemma_evict_elem_tid ep tl
       )
     else
-      IntT.lemma_evict_elem_unique tl (i1 - S.length es') (i2 - S.length es')
+      IntT.lemma_evict_elem_unique ep tl (i1 - S.length es') (i2 - S.length es')
 
-let lemma_evict_elem_unique #vcfg (gl: verifiable_log vcfg) (i1 i2: SA.seq_index (evict_seq gl))
+let lemma_evict_elem_unique #vcfg (ep: epoch) (gl: verifiable_log vcfg) (i1 i2: SA.seq_index (evict_seq ep gl))
   : Lemma (requires (i1 <> i2))
-          (ensures (diff_elem (evict_seq gl) i1 i2))
-          [SMTPat (diff_elem (evict_seq gl) i1 i2)] = 
+          (ensures (diff_elem (evict_seq ep gl) i1 i2))
+          [SMTPat (diff_elem (evict_seq ep gl) i1 i2)] =
   if i1 < i2 then
-    lemma_evict_elem_unique_aux gl i1 i2
+    lemma_evict_elem_unique_aux ep gl i1 i2
   else
-    lemma_evict_elem_unique_aux gl i2 i1
+    lemma_evict_elem_unique_aux ep gl i2 i1
 
-let lemma_evict_elem_unique2 #vcfg (gl: verifiable_log vcfg):
-  Lemma (uniq_prop (evict_seq gl)) = ()
+let lemma_evict_elem_unique2 #vcfg (ep: epoch) (gl: verifiable_log vcfg):
+  Lemma (uniq_prop (evict_seq ep gl)) = ()
 
-let lemma_evict_elem_count #vcfg (gl: verifiable_log vcfg) (x: ms_hashfn_dom)
-  : Lemma (count x (evict_seq gl) <= 1) =
-  lemma_evict_elem_unique2 gl;
-  lemma_uniq_prop_counts (evict_seq gl) x
+let lemma_evict_elem_count #vcfg (ep: epoch) (gl: verifiable_log vcfg) (x: ms_hashfn_dom)
+  : Lemma (count x (evict_seq ep gl) <= 1) =
+  lemma_evict_elem_unique2 ep gl;
+  lemma_uniq_prop_counts (evict_seq ep gl) x
 
 
 module MS = Veritas.MultiSet
 
 (* the global evict set is a set (not a multiset) *)
-let evict_set_is_set (#vcfg:_) (gl: verifiable_log vcfg): 
-  Lemma (ensures (is_set (evict_set gl))) = 
-  let es = evict_set gl in
+let evict_set_is_set (#vcfg:_) (ep: epoch) (gl: verifiable_log vcfg):
+  Lemma (ensures (is_set (evict_set ep gl))) =
+  let es = evict_set ep gl in
   let aux (x:ms_hashfn_dom):
     Lemma (ensures (MS.mem x es <= 1))
           [SMTPat (MS.mem x es)] = 
-      lemma_evict_elem_count gl x;
-      seq2mset_mem #_ #ms_hashfn_dom_cmp (evict_seq gl) x
+      lemma_evict_elem_count ep gl x;
+      seq2mset_mem #_ #ms_hashfn_dom_cmp (evict_seq ep gl) x
   in
   ()
 
-
-let rec evict_seq_map_aux (#vcfg:_) (gl: verifiable_log vcfg) (ii: sseq_index gl {is_evict_to_blum (indexss gl ii)}):
-  Tot (j: SA.seq_index (evict_seq gl) {S.index (evict_seq gl) j = blum_evict_elem gl ii})
+let rec evict_seq_map (#vcfg:_) (gl: verifiable_log vcfg) (ii: sseq_index gl {is_evict_to_blum (indexss gl ii)}):
+  Tot (let e = indexss gl ii in
+   let be = blum_evict_elem gl ii in
+   let ep = epoch_of be in
+   let es = evict_seq ep gl in
+   j: SA.seq_index es {S.index es j = be})
   (decreases (S.length gl)) =
   let (tid, i) = ii in
+  let e = indexss gl ii in
+  let be = blum_evict_elem gl ii in
+  let ep = epoch_of be in
+
   let p = S.length gl in
   let gl' = SA.prefix gl (p - 1) in
-  let s' = evict_seq gl' in
-  let s = evict_seq gl in
+  let s' = evict_seq ep gl' in
   let tl = thread_log gl (p - 1) in
-  let et = IntT.blum_evict_seq tl in
-  if tid = p - 1 then (
-    //S.length s' + IntT.evict_seq_map tl i
-    assert(s == append s' et);
-    assert(S.length s = S.length s' + S.length et);
-    let i' = IntT.evict_seq_map tl i in
-    assert(i' < S.length et);
-    let j = S.length s' + i' in
-    assert(j < S.length s);
-    //assert(S.index s j = blum_evict_elem gl ii);
-    assert(blum_evict_elem gl ii = IntT.blum_evict_elem tl i);
-    assert(IntT.blum_evict_elem tl i = S.index et i');
-    assert(S.index s j = S.index et i');
-    j
-  )
+
+  if tid = p - 1 then
+    S.length s' + IntT.evict_seq_map tl i
   else
-    evict_seq_map_aux gl' ii
+    evict_seq_map gl' ii
 
-let evict_seq_map (#vcfg:_) (gl: verifiable_log vcfg) (ii: sseq_index gl {is_evict_to_blum (indexss gl ii)}):
-  (j: SA.seq_index (evict_seq gl) {S.index (evict_seq gl) j = 
-                                 blum_evict_elem gl ii}) = evict_seq_map_aux gl ii
-
-//#push-options "--z3rlimit_factor 3"
-
-let rec evict_seq_map_inv_aux (#vcfg:_) (gl: verifiable_log vcfg) (j: SA.seq_index (evict_seq gl)):
-  Tot (ii: sseq_index gl {is_evict_to_blum (indexss gl ii) /\
-                      blum_evict_elem gl ii = S.index (evict_seq gl) j /\
-                      evict_seq_map gl ii = j}) 
+let rec evict_seq_map_inv (#vcfg:_) (ep: epoch) (gl: verifiable_log vcfg) (j: SA.seq_index (evict_seq ep gl)):
+  Tot (ii: sseq_index gl {let e = indexss gl ii in
+                      is_evict_to_blum e /\
+                      (let be = blum_evict_elem gl ii in
+                       let es = evict_seq ep gl in
+                       be = S.index es j /\
+                       ep = epoch_of be /\
+                       evict_seq_map gl ii = j)})
   (decreases (S.length gl)) =
   let p = S.length gl in
   let gl' = SA.prefix gl (p - 1) in
-  let s' = evict_seq gl' in
-  let s = evict_seq gl in
+  let s' = evict_seq ep gl' in
   let tl = thread_log gl (p - 1) in
-  let et = IntT.blum_evict_seq tl in
   if j < S.length s' then
-    evict_seq_map_inv_aux gl' j
+    evict_seq_map_inv ep gl' j
   else
     let j' = j - S.length s' in
-    let i = IntT.evict_seq_inv_map tl j' in
-    let ii = (p - 1, i) in
-    assert(s == append s' et);
-    assert(S.index s j = S.index et j');
+    let i = IntT.evict_seq_inv_map ep tl j' in
     (p-1, i)
 
-
-let evict_seq_map_inv (#vcfg:_) (gl: verifiable_log vcfg) (j: SA.seq_index (evict_seq gl)):
-  (ii: sseq_index gl {is_evict_to_blum (indexss gl ii) /\
-                      blum_evict_elem gl ii = S.index (evict_seq gl) j /\
-                      evict_seq_map gl ii = j}) = evict_seq_map_inv_aux gl j
 #push-options "--z3rlimit_factor 2"
-let rec lemma_evict_seq_inv_aux (#vcfg:_) (gl: verifiable_log vcfg) (ii: sseq_index gl {is_evict_to_blum (indexss gl ii)}):
-  Lemma (ensures (evict_seq_map_inv gl (evict_seq_map gl ii) = ii)) 
-        (decreases (S.length gl)) = 
+
+let rec lemma_evict_seq_inv (#vcfg:_) (gl: verifiable_log vcfg)
+  (ii: sseq_index gl {is_evict_to_blum (indexss gl ii)}):
+  Lemma (ensures (let e = indexss gl ii in
+                  let be = blum_evict_elem gl ii in
+                  let ep = epoch_of be in
+                  let j = evict_seq_map gl ii in
+                  evict_seq_map_inv ep gl j = ii))
+        (decreases (S.length gl)) =
+  let e = indexss gl ii in
+  let be = blum_evict_elem gl ii in
+  let ep = epoch_of be in
+
   let (tid, i) = ii in
   let p = S.length gl in
   let gl' = SA.prefix gl (p - 1) in
-  let s' = evict_seq gl' in
+  let s' = evict_seq ep gl' in
   let tl = thread_log gl (p - 1) in
   if tid = p - 1 then ()
   else
-    lemma_evict_seq_inv_aux gl' ii
+    lemma_evict_seq_inv gl' ii
+
 #pop-options
 
-let lemma_evict_seq_inv (#vcfg:_) (gl: verifiable_log vcfg) (ii: sseq_index gl {is_evict_to_blum (indexss gl ii)}):
-  Lemma (requires True)
-        (ensures (evict_seq_map_inv gl (evict_seq_map gl ii) = ii)) = lemma_evict_seq_inv_aux gl ii
+let hadd_hevict_equal (#vcfg:_) (epmax: epoch) (gl: hash_verifiable_log vcfg epmax) (ep: epoch{ep <= epmax}):
+  Lemma (ensures (hadd gl ep = hevict gl ep /\
+                  ms_hashfn (add_seq ep gl) = ms_hashfn (evict_seq ep gl))) =
+  assert(hash_verifiable_prop gl epmax ep);
+  lemma_ghevict_correct ep gl;
+  lemma_g_hadd_correct ep gl
+
+let rec prefix_upto_epoch (#vcfg:_) (ep: epoch) (gl: verifiable_log vcfg)
+  : Tot (gl': verifiable_log vcfg {S.length gl = S.length gl' })
+  (decreases (S.length gl)) =
+
+  let p = S.length gl in
+  if p = 0 then S.empty #(logS vcfg)
+  else (
+    let gl' = SA.prefix gl (p - 1) in
+    let pgl' = prefix_upto_epoch ep gl' in
+    let _, lep = IntT.prefix_upto_epoch ep (thread_log gl (p - 1)) in
+    let pgl = append1 pgl' lep in
+    let aux (tid: SA.seq_index pgl):
+      Lemma (ensures (IntT.verifiable (thread_log pgl tid)))
+            [SMTPat (thread_log pgl tid)] =
+      if tid = p - 1 then ()
+      else
+        assert(thread_log pgl tid = thread_log pgl' tid)
+    in
+    pgl
+  )
+
+let rec lemma_prefix_upto_epoch (#vcfg:_) (ep: epoch) (gl: verifiable_log vcfg) (tid: SA.seq_index gl):
+  Lemma (ensures (let tl = thread_log gl tid in
+                  let _, l_ep = IntT.prefix_upto_epoch ep tl in
+                  let gl_ep = prefix_upto_epoch ep gl in
+                  l_ep = S.index gl_ep tid))
+  (decreases (S.length gl)) =
+  let n = S.length gl in
+  assert(n > 0);
+
+  if tid = n - 1 then ()
+  else
+    lemma_prefix_upto_epoch ep (SA.prefix gl (n - 1)) tid
